doc-src/TutorialI/Types/Overloading2.thy
@@ -23,7 +23,7 @@ subsubsection{*Predefined Overloading*}
 text{*
 HOL comes with a number of overloaded constants and corresponding classes.
 The most important ones are listed in Table~\ref{tab:overloading}. They are
-defined on all numeric types and somtimes on other types as well, for example
+defined on all numeric types and sometimes on other types as well, for example
 @{text"-"}, @{text"\<le>"} and @{text"<"} on sets.
 
 \begin{table}[htbp]
@@ -34,9 +34,13 @@ Constant & Type & Syntax \\
 @{term 0} & @{text "'a::zero"} \\
 @{text"+"} & @{text "('a::plus) \<Rightarrow> 'a \<Rightarrow> 'a"} & (infixl 65) \\
 @{text"-"} & @{text "('a::minus) \<Rightarrow> 'a \<Rightarrow> 'a"} &  (infixl 65) \\
-@{text"*"} & @{text "('a::times) \<Rightarrow> 'a \<Rightarrow> 'a"} & (infixl 70) \\
-@{text"^"} & @{text "('a::power) \<Rightarrow> nat \<Rightarrow> 'a"} & (infixr 80) \\
 @{text"-"} & @{text "('a::minus) \<Rightarrow> 'a"} \\
+@{text"*"} & @{text "('a::times) \<Rightarrow> 'a \<Rightarrow> 'a"} & (infixl 70) \\
+@{text div} & @{text "('a::div) \<Rightarrow> 'a \<Rightarrow> 'a"} & (infixl 70) \\
+@{text mod} & @{text "('a::div) \<Rightarrow> 'a \<Rightarrow> 'a"} & (infixl 70) \\
+@{text dvd} & @{text "('a::times) \<Rightarrow> 'a \<Rightarrow> bool"} & (infixl 50) \\
+@{text"/"}  & @{text "('a::inverse) \<Rightarrow> 'a \<Rightarrow> 'a"} & (infixl 70) \\
+@{text"^"} & @{text "('a::power) \<Rightarrow> nat \<Rightarrow> 'a"} & (infixr 80) \\
 @{term abs} &  @{text "('a::minus) \<Rightarrow> 'a"} & ${\mid} x {\mid}$\\
 @{text"\<le>"} & @{text "('a::ord) \<Rightarrow> 'a \<Rightarrow> bool"} & (infixl 50) \\
 @{text"<"} & @{text "('a::ord) \<Rightarrow> 'a \<Rightarrow> bool"} & (infixl 50) \\
